Adding abstract ID type

src/Eqb_Evidence.v
@@ -1,8 +1,8 @@
-Require Import Term_Defs.
+Require Import AbstractedTypes EqClass Term_Defs.
 
 Require Import StructTactics.
 
-Require Import Coq.Program.Tactics Coq.Bool.Bool.
+Require Import Coq.Program.Tactics.
 Require Import PeanoNat.
 
 (*
@@ -10,109 +10,117 @@ Set Nested Proofs Allowed.
  *)
 
 
-Definition eqb_aspid (a1 a2 : ASP_ID) : bool :=
-  String.eqb a1 a2.
+Definition eqb_aspid `{H : EqClass ID_Type} (a1 a2 : ASP_ID)  : bool :=
+  eqb a1 a2.
 
 (** Admitted Lemmas relating boolean to propositional equality for 
    ASP ID and PARAMS *)
-Lemma eqb_eq_aspid: forall i1 i2,
-    eqb_aspid i1 i2 = true <-> i1 = i2.
+Lemma eqb_eq_aspid: forall `{H : EqClass ID_Type} i1 i2,
+    eqb_aspid i1 i2 = true -> i1 = i2.
 Proof.
-  intros.
-  destruct (eqb_aspid i1 i2) eqn:E.
-  - split; auto. intros. unfold eqb_aspid in E.
-    rewrite String.eqb_eq in E. auto.
-  - split; try congruence. intros.
-    unfold eqb_aspid in E. rewrite String.eqb_neq in E.
-    congruence.
+  unfold eqb_aspid.
+  destruct H. eapply eqb_leibniz.
 Qed.
 
-Open Scope list.
-
-Fixpoint eqb_list_args (a1 a2 : list Arg) : bool :=
-  match a1, a2 with
-  | h1 :: t1, h2 :: t2 => andb (String.eqb h1 h2) (eqb_list_args t1 t2)
-  | nil, nil => true
-  | _, _ => false
-  end.
-
-Close Scope list.
-
-
-Lemma eqb_list_args_true_iff : forall a1 a2,
-    eqb_list_args a1 a2 = true <->
-    a1 = a2.
-Proof.
-  split; intros.
-  - generalize dependent a2.
-    induction a1; simpl; intros.
-    * destruct a2; auto; try congruence.
-    * destruct a2; auto; try congruence.
-      rewrite andb_true_iff in H. destruct_conjs.
-      rewrite String.eqb_eq in H. subst. 
-      apply IHa1 in H0. subst. auto.
-  - subst. induction a2; auto. 
-    simpl; rewrite IHa2. rewrite String.eqb_refl. auto.
-Qed.
-
-Definition eqb_asp_params (ap1 ap2 : ASP_PARAMS) : bool :=
+Definition eqb_asp_params `{H : EqClass ID_Type} `{H : EqClass (list ID_Type)} (ap1 ap2 : ASP_PARAMS) : bool :=
   match ap1, ap2 with
   | (asp_paramsC a1 la1 p1 t1), (asp_paramsC a2 la2 p2 t2) =>
       andb (eqb_aspid a1 a2) 
-        (andb (eqb_list_args la1 la2)
-          (andb (Nat.eqb p1 p2) 
-                (String.eqb t1 t2)))
+        (andb (eqb la1 la2)
+          (andb (eqb p1 p2) 
+                (eqb t1 t2)))
   end.
 
 (** Decidable equality proofs for various Copland datatypes *)
-Definition eq_asp_params_dec:
+Definition eq_asp_params_dec `{H : EqClass ID_Type} :
   forall x y: ASP_PARAMS, {x = y} + {x <> y}.
 Proof.
   intros.
-  decide equality; repeat (decide equality).
+  decide equality; subst;
+  eapply EqClass_impl_DecEq; eauto.
+  eapply EqClass_extends_to_list; eauto.
 Defined.
 
-Lemma eqb_eq_asp_params: forall a a0,
+Lemma eqb_eq_asp_params: forall `{H : EqClass ID_Type} a a0 ,
     eqb_asp_params a a0 = true <->
     a = a0.
 Proof.
-  split; intros; pose proof (eq_asp_params_dec a a0) as HD.
-  - destruct HD; auto. 
-    unfold eqb_asp_params in H.
-    destruct a, a0. 
-    repeat rewrite andb_true_iff in H.
-    destruct_conjs.
-    rewrite String.eqb_eq in *. subst.
-    rewrite Nat.eqb_eq in *. subst.
-    rewrite eqb_list_args_true_iff in *. subst.
-    reflexivity.
-  - subst. unfold eqb_asp_params.
-    destruct a0. 
-    repeat rewrite andb_true_iff.
-    repeat split.
-    * unfold eqb_aspid. rewrite String.eqb_eq. auto.
-    * apply eqb_list_args_true_iff. auto.
-    * rewrite Nat.eqb_eq. auto.
-    * rewrite String.eqb_eq. auto.
+  induction a; destruct a0; simpl;
+  repeat (rewrite Bool.andb_true_iff);
+  repeat split; eauto; try inv H0;
+  try rewrite eqb_leibniz; eauto;
+  try (eapply EqClass_extends_to_list; eauto).
+  - intros; destruct_conjs; subst.
+    repeat (rewrite eqb_leibniz in *); subst.
+    eapply general_list_eqb_leibniz in H1; subst; eauto.
+  - eapply eqb_leibniz; eauto.
 Qed.
 
+Global Instance EqClassASP_PARAMS `{H : EqClass ID_Type} : EqClass ASP_PARAMS := {
+  eqb := eqb_asp_params ;
+  eqb_leibniz := eqb_eq_asp_params
+}.
 
-Definition eq_ev_dec:
+Definition eq_evidence_dec : forall `{H : EqClass ID_Type},
+  forall x y : Evidence, {x = y} + {x <> y}.
+Proof.
+  intros.
+  decide equality; subst;
+  try (try eapply EqClass_impl_DecEq; eauto;
+  try eapply nat_EqClass; eauto; fail).
+  - eapply eq_asp_params_dec.
+  - destruct f, f0; eauto; right; intros HC; congruence.
+Qed.
+
+Definition eq_term_dec : forall `{H : EqClass ID_Type},
+  forall x y : Term, {x = y} + {x <> y}.
+Proof.
+  intros.
+  decide equality; subst;
+  try (try eapply EqClass_impl_DecEq; eauto;
+  try eapply nat_EqClass; eauto; fail).
+  - destruct a, a0; eauto; try (right; intros HC; congruence).
+    * destruct (eq_asp_params_dec a a0); subst; eauto;
+      destruct s, s0, f, f0; eauto; try (right; intros HC; congruence).
+    * destruct (@EqClass_impl_DecEq Plc H p p0); subst; eauto.
+      right; intros HC; congruence.
+  - destruct s, s0, s, s1, s0, s2; eauto; try (right; intros HC; congruence).
+  - destruct s, s0, s, s1, s0, s2; eauto; try (right; intros HC; congruence).
+Qed.
+
+Definition eq_core_term_dec : forall `{H : EqClass ID_Type},
+  forall x y : Core_Term, {x = y} + {x <> y}.
+Proof.
+  intros.
+  decide equality; subst;
+  try (try eapply EqClass_impl_DecEq; eauto;
+  try eapply nat_EqClass; eauto; fail).
+  - destruct a, a0; eauto; try (right; intros HC; congruence).
+    * destruct (eq_asp_params_dec a a0); subst; eauto;
+      destruct f, f0; eauto; try (right; intros HC; congruence).
+  - eapply eq_term_dec.
+Qed.
+
+Definition eq_ev_dec: forall `{H : EqClass ID_Type},
   forall x y: Ev, {x = y} + {x <> y}.
 Proof.
   intros;
-    repeat decide equality;
-    try (apply eq_arg_dec).
-Defined.
+  decide equality; subst;
+  try (try eapply EqClass_impl_DecEq; eauto;
+  try eapply nat_EqClass; 
+  try eapply EqClassASP_Params; eauto; fail).
+  repeat decide equality; subst;
+  try (try eapply EqClass_impl_DecEq; eauto;
+  try eapply nat_EqClass; eauto; fail).
+  - eapply eq_asp_params_dec.
+  - eapply eq_evidence_dec.
+  - eapply eq_term_dec.
+  - eapply eq_evidence_dec.
+  - eapply eq_evidence_dec.
+  - eapply eq_core_term_dec.
+Qed.
 #[local] Hint Resolve eq_ev_dec : core.
 
-Definition eq_evidence_dec:
-  forall x y: Evidence, {x = y} + {x <> y}.
-Proof.
-  intros;
-    repeat decide equality;
-  apply eq_arg_dec.
-Defined.
 #[local] Hint Resolve eq_evidence_dec : core.
 
 
@@ -165,7 +173,7 @@ Proof.
     +
       assert (f a a0 = true /\ list_beq A f x y = true).
       {
-        eapply andb_true_iff.
+        eapply Bool.andb_true_iff.
         eassumption.
       }
       destruct_conjs.
@@ -228,7 +236,7 @@ Proof.
 Admitted.
 
 (** Boolean equality for Evidence Types *)
-Fixpoint eqb_evidence (e:Evidence) (e':Evidence): bool :=
+Fixpoint eqb_evidence `{H : EqClass ID_Type} (e:Evidence) (e':Evidence): bool :=
   match (e,e') with
   | (mt,mt) => true
                 (*
@@ -238,8 +246,8 @@ Fixpoint eqb_evidence (e:Evidence) (e':Evidence): bool :=
     (Nat.eqb p p') && (eqb_asp_params params params') && (eqb_evidence e1 e2)
                  *)
   | (uu p fwd params e1, uu p' fwd' params' e2) =>
-    (Nat.eqb p p') && (eqb_fwd fwd fwd') && (eqb_asp_params params params') && (eqb_evidence e1 e2)
-  | (nn i, nn i') => (Nat.eqb i i')
+    (eqb p p') && (eqb_fwd fwd fwd') && (eqb_asp_params params params') && (eqb_evidence e1 e2)
+  | (nn i, nn i') => (eqb i i')
   | (ss e1 e2, ss e1' e2') =>
     (eqb_evidence e1 e1') && (eqb_evidence e2 e2')
   | _ => false
@@ -257,18 +265,13 @@ Proof.
     generalizeEverythingElse e1.
     induction e1; destruct e2; intros;
       try (cbn in *; repeat break_match; try solve_by_inversion; eauto).
-    +
-      apply EqNat.beq_nat_true in H.
-      eauto.
-
-
-    +
-      cbn in *.
+    + rewrite Nat.eqb_eq in H; eauto.
+    + cbn in *.
       rewrite Bool.andb_true_iff in H.
       rewrite Bool.andb_true_iff in H.
       rewrite Bool.andb_true_iff in H.
       destruct_conjs.
-      apply EqNat.beq_nat_true in H.
+      rewrite eqb_leibniz in H.
       specialize IHe1 with e2.
       concludes.
       rewrite eqb_eq_asp_params in H1.
@@ -320,19 +323,15 @@ Proof.
     generalizeEverythingElse e1.
     induction e1; destruct e2; intros;
       try (cbn in * ; repeat break_match; try solve_by_inversion; eauto).
-    +
-      invc H.
-      apply Nat.eqb_refl.
-      
-    +
-      invc H.
+    + invc H. rewrite Nat.eqb_eq; eauto.
+    + invc H.
       cbn in *.
       repeat rewrite Bool.andb_true_iff.
-      split. split. split.
-      apply Nat.eqb_refl.
-      rewrite eqb_eq_fwd. tauto.
-      erewrite eqb_eq_asp_params. tauto.
-      eauto.
+      split. split. split. 
+      * eapply eqb_leibniz; eauto.
+      * rewrite eqb_eq_fwd. tauto.
+      * erewrite eqb_eq_asp_params. tauto.
+      * eauto.
       (*
     +
       invc H.
